
########################################################################################
#                                                                                      #
#        Branch of VISO for (RoMM-)ATOMISTIC AND (RoMM-)MESOSCOPIC MODELS/SOLVERS      #
#                                                                                      #
########################################################################################

@prefix viso: <https://purl.vimmp.eu/semantics/viso/viso-general.ttl#>.
@prefix viso-am: <https://purl.vimmp.eu/semantics/viso/viso-atomistic-mesoscopic.ttl#>.
@prefix vov: <https://purl.vimmp.eu/semantics/vov/vov.ttl#>.

@prefix owl: <http://www.w3.org/2002/07/owl#>.
@prefix rdf: <http://www.w3.org/1999/02/22-rdf-syntax-ns#>.
@prefix rdfs: <http://www.w3.org/2000/01/rdf-schema#>.
@prefix xs: <http://www.w3.org/2001/XMLSchema#>.
@prefix dcterms: <http://purl.org/dc/terms/>.

<https://purl.vimmp.eu/semantics/viso/viso-atomistic-mesoscopic.ttl#> a owl:Ontology.

############################  Ontology header  #########################################

<https://purl.vimmp.eu/semantics/viso/viso-atomistic-mesoscopic.ttl#>
  owl:imports <https://purl.vimmp.eu/semantics/viso/viso-general.ttl#>;
  dcterms:title "VISO-AM: Branch of VISO for (RoMM-)Atomistic and (RoMM-)Mesoscopic models/solvers"^^xs:string;
  dcterms:modified "2020-06-18"^^xs:string;
  dcterms:creator "Silvia Chiacchiera (ORCID 0000-0003-0422-7870)"^^xs:string;
  dcterms:creator "Martin T. Horsch (ORCID 0000-0002-9464-6739)"^^xs:string;
  dcterms:creator "Mara Chiricotto (ORCID 0000-0003-1609-5254)"^^xs:string;
  dcterms:creator "Michael A. Seaton (ORCID 0000-0002-4708-573X)"^^xs:string;
  dcterms:creator "Ilian T. Todorov (ORCID 0000-0001-7275-1784)"^^xs:string;
  dcterms:creator "Gianluca Boccardo (ORCID 0000-0003-1264-8237)"^^xs:string;
  dcterms:creator "Joshua D. Elliott (ORCID 0000-0002-0729-246X)"^^xs:string;
  dcterms:contributor "Welchy Leite Cavalcanti"^^xs:string;
  dcterms:contributor "Gerhard Goldbeck (ORCID 0000-0002-4181-2852)"^^xs:string;
  dcterms:contributor "Daniele Toti (ORCID 0000-0002-9668-6961)"^^xs:string;	
  dcterms:license "GNU Lesser General Public License (LGPL) version 3"^^xs:string;
  dcterms:description """VISO-AM expands on the model types, model and solver features for 
Atomisitic and Mesoscopic (as per RoMM) models."""^^xs:string;
  dcterms:bibliographicCitation "10.1021/acs.jced.9b00739"^^xs:string;
  rdfs:comment """The authors acknowledge funding from the European Union's Horizon 2020 research and
innovation programme under grant agreement no. 760907, Virtual Materials Marketplace (VIMMP)."""^^xs:string.
  
##############  Atomistic and Mesoscopic model types ##################################

viso-am:molecular_dynamics a owl:Class; 
  rdfs:subClassOf viso:am_model_type;
  rdfs:comment "Molecular Dynamics."^^xs:string;
  rdfs:subClassOf viso:R_IS_ATOMISTIC;
  rdfs:subClassOf viso:R_IS_MESOSCOPIC.

viso-am:molecular_mechanics a owl:Class;
  rdfs:subClassOf viso:am_model_type;
  rdfs:comment "Molecular Mechanics or Molecular Statics."^^xs:string;
  rdfs:subClassOf viso:R_IS_ATOMISTIC;
  rdfs:subClassOf viso:R_IS_MESOSCOPIC.
      
viso-am:molecular_monte_carlo a owl:Class; 
  rdfs:subClassOf viso:am_model_type;
  rdfs:comment "Molecular Monte Carlo method."^^xs:string;
  rdfs:subClassOf viso:R_IS_ATOMISTIC;
  rdfs:subClassOf viso:R_IS_MESOSCOPIC.

viso-am:dissipative_particle_dynamics a owl:Class; 
  rdfs:subClassOf viso:am_model_type;
  rdfs:comment "Dissipative Particle Dynamics."^^xs:string;
  rdfs:subClassOf viso:R_IS_MESOSCOPIC.

viso-am:MD a viso-am:molecular_dynamics;
   viso:has_osmo_pe_type_id "A.3";
   viso:has_osmo_pe_type_id "M.3";
   viso:has_pe viso-am:NEWTON_EQUATION.

viso-am:MM a viso-am:molecular_mechanics;
   viso:has_osmo_pe_type_id "A.2";
   viso:has_osmo_pe_type_id "M.2".	
   
viso-am:MC a viso-am:molecular_monte_carlo;
   viso:has_osmo_pe_type_id "A.4";
   viso:has_osmo_pe_type_id "M.4";
   viso:has_pe viso-am:PHASE_SPACE_SAMPLING_EQUATION.

viso-am:DPD a viso-am:dissipative_particle_dynamics;
  viso:has_osmo_pe_type_id "M.3";
  viso:has_pe viso-am:NEWTON_EQUATION_PLUS_RANDOM_AND_DRAG_FORCE. 

##############  Connection of model_type to model_object  #############################

viso:am_model_type rdfs:subClassOf [a owl:Restriction;
  		  owl:onProperty vov:involves_object;
		  owl:someValuesFrom viso-am:interaction_site].

##############  Atomistic and Mesoscopic solver feature ###############################
viso-am:thermostat a owl:Class;
  rdfs:subClassOf viso:am_solver_feature.

viso-am:barostat a owl:Class;
  rdfs:subClassOf viso:am_solver_feature.

viso-am:integrator a owl:Class;
  rdfs:subClassOf viso:am_solver_feature;
  rdfs:comment "An algorithm to integrate Newton second law."^^xs:string.

viso-am:minimization a owl:Class;
  rdfs:subClassOf viso:am_solver_feature;
  rdfs:comment "An algorithm for energy minimization/geometry optimization."^^xs:string.

viso-am:electrostatics_solver a owl:Class;
  rdfs:subClassOf viso:am_solver_feature.

viso-am:parallelization_scheme a owl:Class;
  rdfs:subClassOf viso:am_solver_feature.

viso-am:geometric_constraint_algorithm a owl:Class;
  rdfs:subClassOf viso:am_solver_feature.

viso-am:sampling_algorithm a owl:Class;
  rdfs:subClassOf viso:am_solver_feature.

viso-am:charge_smearing a owl:Class;
  rdfs:subClassOf viso:am_solver_feature;
  rdfs:comment "Charge smearing is sometimes used in combination with soft potentials (e.g., dpd potential) to avoid the divergence of the interaction energy of opposite charges."^^xs:string.

##############  (6) model feature ################################

viso-am:NEWTON_EQUATION a viso:am_physical_equation;
 rdfs:comment "Newton's second law of motion."^^xs:string.

viso-am:NEWTON_EQUATION_PLUS_RANDOM_AND_DRAG_FORCE a viso:am_physical_equation;
 rdfs:comment """Newton's second law of motion, with explicit terms for the DPD thermostat (random and drag force terms). The splitting into PE and MR for this case can be debated, as the thermostat affects the material transport properties. Here we choose to put in the MR part the conservative forces only."""^^xs:string.

viso-am:PHASE_SPACE_SAMPLING_EQUATION a viso:am_physical_equation;
 rdfs:comment "We indicate as Phase-Space Sampling equation any equation that allows to generate configurations (i.e., microstates) according to a given ensemble (macrostate)."^^xs:string.

viso:am_external_condition_trait a owl:Class;
  rdfs:subClassOf viso:am_model_feature.

viso-am:external_field a owl:Class;
  rdfs:subClassOf viso:am_external_condition_trait.

viso-am:external_conservative_field a owl:Class;
  rdfs:subClassOf viso-am:external_field;
  rdfs:subClassOf [a owl:Restriction;
      owl:onProperty viso:is_mathematically_related_to;
      owl:minQualifiedCardinality 1;
      owl:onClass viso-am:external_potential].

viso-am:external_non_conservative_field a owl:Class;
  rdfs:subClassOf viso-am:external_field.

viso-am:external_field owl:disjointUnionOf (viso-am:external_conservative_field viso-am:external_non_conservative_field).

viso-am:EXTERNAL_ELECTRIC_FIELD a viso-am:external_conservative_field.
viso-am:EXTERNAL_GRAVITY_FIELD a viso-am:external_conservative_field.

viso-am:composite_potential a owl:Class; 
  rdfs:subClassOf viso:am_materials_relation_trait;
  rdfs:comment """A potential that is defined by more than just one single functional form acting between a pair of species. 
  For example, it is the sum of two or more potentials having different functional forms (e.g., a stretching potential and an angle potential) 
  and/or it applies to at least two pairs of species with different parameters (e.g., a Mie potential between species pairs {A,A}, {A,B} and {B,B}). 
  It can contain combination and/or exclusion rules."""^^xs:string;
  rdfs:subClassOf [a owl:Restriction;
    owl:onProperty viso:has_part;
    owl:minQualifiedCardinality 2;
    owl:onClass viso-am:potential].

viso-am:potential a owl:Class; 
  rdfs:subClassOf viso:am_materials_relation_trait;
  rdfs:comment """The mathematical expression (functional form) of a potential energy, i.e., of the energy associated with a conservative force. 
  It is a building block of composite potentials (cf. composite_potential class).
  It can concern both interactions of particles between them and with the external world."""^^xs:string.

viso-am:non_bonding_potential a owl:Class; 
  rdfs:subClassOf viso-am:potential;
  rdfs:comment """A potential defined between particles of given species, that is not associated to bonding and acts between and within molecules. It is commonly switched off for 'closest' particles. Sometimes called 'inter-molecular potential', even if this is strictly correct only for small molecules, not for bigger ones."""^^xs:string.

viso-am:two_body_potential a owl:Class;
  rdfs:subClassOf viso-am:potential.

viso-am:three_body_potential a owl:Class;
  rdfs:subClassOf viso-am:potential.

viso-am:four_body_potential a owl:Class;
  rdfs:subClassOf viso-am:potential.

viso-am:bonding_potential a owl:Class;
  rdfs:subClassOf viso-am:potential;
  rdfs:comment "A potential defined between particles within a molecule. Sometimes called 'intra-molecular' potential."^^xs:string.

viso-am:stretching_potential a owl:Class;
  rdfs:subClassOf viso-am:bonding_potential;
  rdfs:subClassOf viso-am:two_body_potential;	
  rdfs:comment "Bonding two-body potential between particles within a molecule. It is a function of the inter-particle distance."^^xs:string.

viso-am:angle_potential a owl:Class;
  rdfs:subClassOf viso-am:bonding_potential;
  rdfs:subClassOf viso-am:three_body_potential;	
  rdfs:comment "Angular three-body potential between particles within a molecule."^^xs:string.

viso-am:dihedral_potential a owl:Class;
  rdfs:subClassOf viso-am:bonding_potential;
  rdfs:subClassOf viso-am:four_body_potential;
  rdfs:comment "Dihedral four-body potential between particles within a molecule. It describes the interaction arising from torsional forces in molecules. Sometimes referred to as torsion potentials."^^xs:string.

viso-am:improper_potential a owl:Class;
  rdfs:subClassOf viso-am:bonding_potential;
  rdfs:subClassOf viso-am:four_body_potential;
  rdfs:comment "Improper dihedral four-body potential between particles within a molecule. It is used to restrict the geometry of a molecule."^^xs:string.

viso-am:electrostatic_potential a owl:Class;
  rdfs:subClassOf viso-am:non_bonding_potential;
  rdfs:subClassOf viso-am:two_body_potential.

viso-am:mie_potential a owl:Class;
   rdfs:subClassOf viso-am:non_bonding_potential;
   rdfs:subClassOf viso-am:two_body_potential;
   rdfs:comment "Mie n-m potential. It includes the Lennard-Jones potential as a special case."^^xs:string;
   rdfs:seeAlso "Gustav Mie,'Zur kinetischen Theorie der einatomigen Körper', Annalen der Physik 11 pp. 657-697 (1903)."^^xs:string;
   rdfs:seeAlso "J. E. Jones. On the determination of molecular fields. II. From the equation of state of a gas. Proceedings of the Royal Society of London Series A, 106(738):463–477, October 1924."^^xs:string.

viso-am:buckingham a owl:Class;
   rdfs:subClassOf viso-am:non_bonding_potential;
   rdfs:subClassOf viso-am:two_body_potential;
   rdfs:seeAlso "R. A. Buckingham and John Edward Lennard-Jones, The classical equation of state of gaseous helium, neon and argon, Proc. R. Soc. Lond. A., 168, 1938."^^xs:string.

viso-am:hard_sphere_potential a owl:Class;
   rdfs:subClassOf viso-am:non_bonding_potential;
   rdfs:subClassOf viso-am:two_body_potential;
   rdfs:comment "Hard-sphere potential."^^xs:string.

viso-am:dpd_potential a owl:Class;
   rdfs:subClassOf viso-am:non_bonding_potential;
   rdfs:comment "Potential to be used in Dissipative Particle Dynamics simulations."^^xs:string;
   rdfs:subClassOf viso:R_IS_MESOSCOPIC.

viso-am:non_bonding_potential a owl:Class;
 owl:disjointUnionOf  (viso-am:electrostatic_potential viso-am:mie_potential viso-am:buckingham viso-am:metal_potential viso-am:dpd_potential).

viso-am:metal_potential a owl:Class;
  rdfs:subClassOf viso-am:non_bonding_potential.
  
viso-am:external_potential a owl:Class;
  rdfs:subClassOf viso-am:potential;
  rdfs:subClassOf viso:am_external_condition_trait;
  rdfs:subClassOf [a owl:Restriction;
      owl:onProperty viso:is_mathematically_related_to;
      owl:minQualifiedCardinality 1;
      owl:onClass viso-am:external_conservative_field].

viso-am:site_surface_potential a owl:Class;
  rdfs:subClassOf viso-am:potential;
  rdfs:comment "A potential for the interaction between a site and a surface (e.g., between a particle and a wall)."^^xs:string.  

# Force fields

viso-am:force_field a owl:Class; 
  rdfs:comment "A Force Field (FF), despite the name, in some areas (as computational chemistry and molecular simulations) refers to the functional form and parameter sets used to calculate the potential energy of a system of particles (atoms or coarse-grained particles). Families of popular FFs exist: they are typically developed witin a community, for a class of materials and using a certain metodology."^^xs:string;
  rdfs:comment "Called Interatomic Potential in the physics community."^^xs:string;
  rdfs:subClassOf viso-am:composite_potential.

viso-am:opls_ff a owl:Class;
  rdfs:subClassOf viso-am:force_field;
  rdfs:comment "Optimized Potentials for Liquid Simulations (OPLS) is a family of force fields. It contains both All-Atomistic (AA) and United-Atom (UA) force fields."^^xs:string;
  rdfs:seeAlso "Jorgensen WL, Tirado-Rives J (1988). 'The OPLS Force Field for Proteins. Energy Minimizations for Crystals of Cyclic Peptides and Crambin'. J. Am. Chem. Soc. 110 (6): 1657–1666.'. "^^xs:string;
  rdfs:seeAlso "Jorgensen WL, Maxwell DS, Tirado-Rives J (1996). 'Development and Testing of the OPLS All-Atom Force Field on Conformational Energetics and Properties of Organic Liquids'. J. Am. Chem. Soc. 118 (45): 11225–11236."^^xs:string.

viso-am:amber_ff a owl:Class;
  rdfs:comment "Assisted Model Building with Energy Refinement (AMBER) Force Field is a family of force fields. Not to be confused with the related software tool."^^xs:string;
  rdfs:seeAlso "http://ambermd.org/AmberModels.php"^^xs:anyURI;
  rdfs:subClassOf viso-am:force_field.

viso-am:charmm_ff a owl:Class;
  rdfs:comment "Chemistry at Harvard Macromolecular Mechanics (CHARMM) Force Field is a family of force fields. Not to be confused with the related software tool."^^xs:string;
  rdfs:seeAlso "http://mackerell.umaryland.edu/charmm_ff.shtml"^^xs:anyURI;
  rdfs:subClassOf viso-am:force_field.

viso-am:gromos_ff a owl:Class;
  rdfs:comment "GROningen MOlecular Simulation (GROMOS) Force Field is a family of force fields. Not to be confused with the related software tool."^^xs:string;
  rdfs:seeAlso "http://www.gromos.net/page.pl?page=about"^^xs:anyURI;
  rdfs:subClassOf viso-am:force_field.

viso-am:dreiding_ff a owl:Class;
  rdfs:subClassOf viso-am:force_field;
  rdfs:comment "DREIDING is a generic force field for molecular simulations."^^xs:string;  		 
  rdfs:seeAlso "Mayo, S. L., Olafson, B. D., and Goddard, W. A., 1990, J. Phys. Chem., 94, 8897"^^xs:string.

viso-am:uff_ff a owl:Class;
  rdfs:subClassOf viso-am:force_field;
  rdfs:comment "The Universal Force Field (UFF) is a full periodic-table force field."^^xs:string;  		 
  rdfs:seeAlso "A. K. Rappe, C. J. Casewit, K. S. Colwell, W. A. Goddard, W. M. Skiff, 'UFF, a full periodic table force field for molecular mechanics and molecular dynamics simulations', J. Am. Chem. Soc. 114, 10024-10035 (1992)."^^xs:string. 

viso-am:pcff_ff a owl:Class; 
  rdfs:comment "Polycarbonate Compatible Force Field."^^xs:string;
  rdfs:seeAlso "Huai Sun, Stephen J. Mumby, Jon R. Maple, and Arnold T. Hagler, 'An ab Initio CFF93 All-Atom Force Field for Polycarbonates', J. Am. Chem. Soc. 116, 2978-2987 (1994)."^^xs:string; 
  rdfs:subClassOf viso-am:force_field.

viso-am:gaff_ff a owl:Class; 
  rdfs:comment "Generalized AMBER force field."^^xs:string;  		 
  rdfs:seeAlso "Junmei Wang, Romain M. Wolf, James W. Caldwell, Peter A. Kollman, David A. Case, 'Development and testing of a general amber force field',J. Comput. Chem. 25, 1157 (2004)."^^xs:string;  		 
  rdfs:subClassOf viso-am:force_field.

viso-am:aua_ff a owl:Class;
  rdfs:comment "Anisotropic United Atom force field."^^xs:string;  		 
  rdfs:seeAlso "Ungerer et al., J. Chem. Phys. 112(12), 5499-5510, 2000."^^xs:string;
  rdfs:subClassOf viso-am:force_field.

viso-am:trappe_ff a owl:Class;
  rdfs:comment "Transferable Potentials for Phase Equilibria."^^xs:string;  		 
  rdfs:seeAlso "Eggimann et al., Mol. Sim. 40(1-3), 101-105, 2014"^^xs:string;
  rdfs:subClassOf viso-am:force_field.

viso-am:martini_ff a owl:Class;
  rdfs:subClassOf viso-am:force_field;
  rdfs:comment "The Martini force field is a coarse-grained (CG) force field suited for molecular dynamics simulations of biomolecular systems."^^xs:string;
  rdfs:seeAlso "http://cgmartini.nl/index.php"^^xs:anyURI;
  rdfs:seeAlso "S.J. Marrink, H.J. Risselada, S. Yefimov, D.P. Tieleman, A.H. de Vries. 'The MARTINI forcefield: coarse grained model for biomolecular simulations'. J. Phys. Chem. B, 111:7812-7824, 2007."^^xs:string.

viso-am:reaxff_ff a owl:Class;
  rdfs:subClassOf viso-am:force_field;
  rdfs:comment "ReaxFF: A Reactive Force Field for Hydrocarbons."^^xs:string;
  rdfs:seeAlso "van Duin, ACT; Dasgupta, S; Lorant, F; Goddard, WA, 'ReaxFF:  A Reactive Force Field for Hydrocarbons.',  J. Phys. Chem. A 105, 9396-9409 (2001)"^^xs:string.

##################################################################

### Object Properties ###

# MD - DPD specfic property (currently, MD/DPD specific. May be generalized later)

viso-am:has_rule a owl:ObjectProperty;
  rdfs:domain viso-am:composite_potential;
  rdfs:range viso-am:rule;
  rdfs:subPropertyOf viso:has_part.

###################################################################
# More model features #

viso-am:statistical_mechanics_entity a owl:Class;
  rdfs:subClassOf viso:modeling_related_entity.

viso-am:thermodynamic_ensemble a owl:Class;
  rdfs:subClassOf viso-am:statistical_mechanics_entity;
  rdfs:subClassOf viso:am_external_condition_trait.

viso-am:model_object a owl:Class;  
  rdfs:subClassOf viso:am_materials_relation_trait;
  rdfs:subClassOf viso:model_object;  
rdfs:comment "Type of object entering the model (e.g., rigid, flexible, or structureless objects)."^^xs:string;
  owl:disjointUnionOf (viso-am:structureless_object viso-am:composite_object).  

viso-am:composite_object a owl:Class;  
  rdfs:subClassOf viso-am:model_object;
  rdfs:comment """A model object having as parts two or more model objects, which can be connected or not.
  For example: a molecule made of two bonded atoms; a polymer made of bonded monomers; 
  or an unbonded pair made of a negative and a positive ion. 
  Such unconnected objects are sometimes defined for convenience (e.g., to ensure the populations of two 
  species are the same)."""^^xs:string;
  rdfs:subClassOf [a owl:Restriction;
      owl:onProperty viso:has_part;
      owl:minQualifiedCardinality 2;
      owl:onClass viso-am:structureless_object].
		  
viso-am:connected_object a owl:Class;  
  rdfs:subClassOf viso-am:composite_object;
  rdfs:subClassOf [a owl:Restriction; owl:onProperty viso:has_part; owl:someValuesFrom
  		  [a owl:Class; owl:unionOf
  		     ([a owl:Restriction; owl:onProperty viso:is_involved_in; owl:someValuesFrom viso-am:stretching_potential]
		     	 [a owl:Restriction; owl:onProperty viso:is_involved_in; owl:hasValue viso-am:RIGID_BOND])]].

viso-am:unconnected_object a owl:Class;  
  rdfs:subClassOf viso-am:composite_object.

viso-am:rigid_object a owl:Class;  
  rdfs:subClassOf viso-am:connected_object;
  rdfs:subClassOf [a owl:Restriction; owl:onProperty viso:has_part; owl:someValuesFrom
		       	 [a owl:Restriction; owl:onProperty viso:is_involved_in; owl:hasValue viso-am:RIGID_BOND]].

viso-am:flexible_object a owl:Class;  
  rdfs:subClassOf viso-am:connected_object;
  rdfs:subClassOf [a owl:Restriction; owl:onProperty viso:has_part; owl:someValuesFrom
    		  [a owl:Restriction; owl:onProperty viso:is_involved_in; owl:someValuesFrom viso-am:stretching_potential]].

viso-am:structureless_object a owl:Class;  
  rdfs:subClassOf viso-am:model_object.

viso-am:interaction_site a owl:Class;
  rdfs:subClassOf viso-am:structureless_object;
  rdfs:comment """An interaction site is a point which is involved in (experiences) some interaction.
  It can represent the center of a physical particle (an atom, a coarse-grained bead), 
  but also be a ficticious particle."""^^xs:string;
  rdfs:comment """For example: consider three sites, one carries a mass, one an electric charge +q, the other a charge -q. 
  The three sites individually have no physical counterpart; however, combined together, they allow to model an object 
  that has a mass and a charge dipole moment. """^^xs:string.


viso-am:lj_site a owl:Class;
  rdfs:subClassOf viso-am:interaction_site;
    rdfs:subClassOf [a owl:Restriction;
                     owl:onProperty viso:is_involved_in;
		     owl:hasValue viso-am:LENNARD_JONES_12_6].

viso-am:mie_site a owl:Class;
  rdfs:subClassOf viso-am:interaction_site;
  rdfs:subClassOf [a owl:Restriction;
                     owl:onProperty viso:is_involved_in;
		     owl:someValuesFrom viso-am:mie_potential].

viso-am:dpd_site a owl:Class;
  rdfs:subClassOf viso-am:interaction_site;
  rdfs:subClassOf [a owl:Restriction;
                     owl:onProperty viso:is_involved_in;
		     owl:someValuesFrom viso-am:dpd_potential];
  rdfs:comment "It is the center of a DPD bead."^^xs:string.

viso-am:mass_site a owl:Class;
  rdfs:subClassOf viso-am:interaction_site.

viso-am:charge_site a owl:Class;
  rdfs:subClassOf viso-am:interaction_site;
  rdfs:subClassOf [a owl:Restriction;
  		     owl:onProperty viso:is_involved_in;
		     owl:someValuesFrom viso-am:electrostatic_potential].

viso-am:charge_dipole_site a owl:Class;
  rdfs:subClassOf viso-am:interaction_site;
  rdfs:subClassOf [a owl:Restriction;
                     owl:onProperty viso:is_involved_in;
		     owl:someValuesFrom viso-am:electrostatic_potential].

viso-am:charge_quadrupole_site a owl:Class;
  rdfs:subClassOf viso-am:interaction_site;
  rdfs:subClassOf [a owl:Restriction;
                     owl:onProperty viso:is_involved_in;
		     owl:someValuesFrom viso-am:electrostatic_potential].

viso-am:wall_site a owl:Class;
  rdfs:subClassOf viso-am:interaction_site;
  rdfs:subClassOf viso:am_external_condition_trait;
  rdfs:comment "A site that, together with others, forms a boundary wall. Such sites are typically frozen (i.e., their positions are fixed in time)."^^xs:string.

viso-am:interaction_surface a owl:Class;
  rdfs:subClassOf viso-am:structureless_object;
  owl:disjointWith viso-am:interaction_site;
  rdfs:comment "A surface which affects interactions, for example a wall. It is described as a continuum surface, not as a collection of sites."^^xs:string.  

viso-am:interaction_plane a owl:Class;
  rdfs:subClassOf viso-am:interaction_surface;
  rdfs:comment "A planar surface which affects interactions, for example a planar wall."^^xs:string.  

viso-am:planar_wall a owl:Class;
  rdfs:subClassOf viso-am:interaction_plane;
  rdfs:subClassOf viso:am_external_condition_trait;
  rdfs:comment "A planar wall (i.e, a boundary surface). It is described as a continuum, not as a collection of sites."^^xs:string.  

viso-am:geometric_constraint a owl:Class;  
  rdfs:subClassOf viso:am_materials_relation_trait.

viso-am:boundary_condition a owl:Class;
  rdfs:subClassOf viso:am_external_condition_trait.
  
viso-am:rule a owl:Class;
  rdfs:subClassOf viso:am_materials_relation_trait.

viso-am:combination_rule a owl:Class;
  rdfs:subClassOf viso-am:rule;
  rdfs:comment "Combination rules or combining rules are equations that can be used to define the interaction parameters between unlike species combining the like-like ones. They apply to non-bonding forces."^^xs:string.

viso-am:exclusion_rule a owl:Class;
  rdfs:subClassOf viso-am:rule;
  rdfs:comment "Exclusion rules are rules that affect the strength of non-bonding forces within a molecule. In some communities, typically 1-2, 1-3 and 1-4 interactions are switched off or scaled."^^xs:string.

viso-am:non_conservative_force a owl:Class;
  rdfs:subClassOf viso:am_materials_relation_trait;
  rdfs:comment "Non-conservative force, typically appearing in coarse-grained models. For example, random and drag forces in Dissipative Particle Dynamics, that together act as a thermostat."^^xs:string.  
##########   Restrictions on software tools (i.e., minimal solver needs)    ###########

[a owl:Restriction; owl:onProperty viso:is_tool_for_model; owl:hasValue viso-am:MD]
  rdfs:subClassOf [a owl:Restriction;
      owl:onProperty viso:has_feature;
      owl:minQualifiedCardinality 1;      
      owl:onClass viso-am:integrator].

[a owl:Restriction; owl:onProperty viso:is_tool_for_model; owl:hasValue viso-am:MM]
  rdfs:subClassOf [a owl:Restriction;
      owl:onProperty viso:has_feature;
      owl:minQualifiedCardinality 1;      
      owl:onClass viso-am:minimization].

[a owl:Restriction; owl:onProperty viso:is_tool_for_model; owl:hasValue viso-am:MC]
  rdfs:subClassOf [a owl:Restriction;
      owl:onProperty viso:has_feature;
      owl:minQualifiedCardinality 1;      
      owl:onClass viso-am:sampling_algorithm].

########################################################

########################################################

###  INSTANCES DEFINITION and DECLARATION OF DIFFERENCES

# thermodynamic_ensemble 

viso-am:NVE a viso-am:thermodynamic_ensemble.

viso-am:NVT a viso-am:thermodynamic_ensemble.

viso-am:NPT a viso-am:thermodynamic_ensemble.

_:C_THERMODYNAMIC_ENSEMBLE rdf:type owl:AllDifferent;
  owl:distinctMembers (viso-am:NVE viso-am:NVT viso-am:NPT).

# integrator

viso-am:VV a viso-am:integrator;
  rdfs:comment "Velocity-Verlet integrator."^^xs:string.

viso-am:DPD_VV a viso-am:integrator;
  rdfs:comment "Version of Velocity-Verlet integrator adapted to the DPD thermostat."^^xs:string.

viso-am:LFV a viso-am:integrator;
  rdfs:comment "Leapfrog-Verlet integrator."^^xs:string.

_:C_INTEGRATOR rdf:type owl:AllDifferent;
  owl:distinctMembers (viso-am:VV viso-am:DPD_VV viso-am:LFV).

# thermostat

viso-am:DPD_THERMOSTAT a viso-am:thermostat.

viso-am:LOWE_ANDERSEN_THERMOSTAT a viso-am:thermostat;
  rdfs:seeAlso "C. P. Lowe. An alternative approach to dissipative particle dynamics. EPL (Europhysics Letters), 47(2):145–151, July 1999."^^xs:string.

viso-am:PETERS_THERMOSTAT a viso-am:thermostat;
  rdfs:seeAlso "E. A. J. F. Peters. Elimination of time step effects in DPD. EPL (Europhysics Letters), 66(3):311–317, May 2004."^^xs:string.

viso-am:STOYANOV_GROOT_THERMOSTAT a viso-am:thermostat;
  rdfs:seeAlso """Simeon D. Stoyanov and Robert D. Groot. From molecular dynamics to hydrodynamics: A novel Galilean
invariant thermostat. Journal of Chemical Physics, 122(11):114112, 2005."""^^xs:string.


viso-am:BERENDSEN_THERMOSTAT a viso-am:thermostat;
  rdfs:seeAlso """Berendsen, H. J. C., Postma, J. P. M., DiNola, A., Haak, J. R. Molecular dynamics with
  coupling to an external bath. J. Chem. Phys. 81:3684–3690, 1984"""^^xs:string.

viso-am:ANDERSEN_THERMOSTAT a viso-am:thermostat;
  rdfs:seeAlso """Andersen, H. C. Molecular dynamics simulations at constant pressure and/or temperature.
  J. Chem. Phys. 72:2384, 1980"""^^xs:string.

viso-am:NOSE_HOOVER_THERMOSTAT a viso-am:thermostat;
  rdfs:seeAlso """Nose, S. A molecular dynamics method for simulations in the canonical ensemble. Mol. Phys. 52:255–268, 1984
                Hoover, W. G. Canonical dynamics: equilibrium phase-space distributions. Phys. Rev. A 31:1695–1697, 1985"""^^xs:string.

viso-am:VELOCITY_RESCALE_THERMOSTAT a viso-am:thermostat;
  rdfs:seeAlso """Bussi, G., Donadio, D., Parrinello, M. Canonical sampling through velocity rescaling. J.
 Chem. Phys. 126:014101, 2007."""^^xs:string.


_:C_THERMOSTAT rdf:type owl:AllDifferent;
  owl:distinctMembers (viso-am:DPD_THERMOSTAT viso-am:LOWE_ANDERSEN_THERMOSTAT viso-am:PETERS_THERMOSTAT viso-am:STOYANOV_GROOT_THERMOSTAT viso-am:BERENDSEN_THERMOSTAT viso-am:ANDERSEN_THERMOSTAT  viso-am:NOSE_HOOVER_THERMOSTAT viso-am:VELOCITY_RESCALE_THERMOSTAT ).

# minimization

viso-am:STEEPEST_DESCENT a viso-am:minimization;
  rdfs:comment "Steepest descent or gradient descent, not the be confused with the method to approximately compute integrals."^^xs:string;
  rdfs:seeAlso "W. H. Press et al, Numerical recipes: The art of scientific computing, 3rd edition, Cambridge University Press, 2007."^^xs:string.

viso-am:CONJUGATE_GRADIENT a viso-am:minimization;
  rdfs:seeAlso "W. H. Press et al, Numerical recipes: The art of scientific computing, 3rd edition, Cambridge University Press, 2007."^^xs:string.

viso-am:BFGS a viso-am:minimization;
  rdfs:comment "Broyden-Fletcher-Goldfarb-Shanno (BFGS) method."^^xs:string;
  rdfs:seeAlso "W. H. Press et al, Numerical recipes: The art of scientific computing, 3rd edition, Cambridge University Press, 2007."^^xs:string.

_:C_MINIMIZATION rdf:type owl:AllDifferent;
  owl:distinctMembers (viso-am:STEEPEST_DESCENT viso-am:CONJUGATE_GRADIENT viso-am:BFGS).

# electrostatic_solver

viso-am:DIRECT_COULOMB_SUM a viso-am:electrostatics_solver.

viso-am:EWALD a viso-am:electrostatics_solver;
  rdfs:comment "Standard Ewald summation method for electrostatics of point-like charges."^^xs:string. 

viso-am:EWALD_SMEARED a viso-am:electrostatics_solver;
  rdfs:comment "Ewald summation method for electrostatics modified to treat smeared charges."^^xs:string;
  rdfs:seeAlso "Minerva González-Melchor, Estela Mayoral, Marı́a Eugenia Velázquez, and José Alejandre. Electro-static interactions in dissipative particle dynamics using the Ewald sums. Journal of Chemical Physics,125(22):224107, 2006."^^xs:string.

viso-am:SPME a viso-am:electrostatics_solver;
   rdfs:comment "Smooth Particle Mesh Ewald summation method for electrostatics. Applies to periodic systems."^^xs:string;
   rdfs:seeAlso "Ulrich Essmann, Lalith Perera, Max L. Berkowitz, Tom Darden, Hsing Lee, and Lee G. Pedersen. A smooth particle mesh Ewald method. J. Chem. Phys. 103, 8577 (1995)."^^xs:string.

viso-am:P3M a viso-am:electrostatics_solver;
   rdfs:comment "Particle-particle particle-mesh summation method for electrostatics."^^xs:string.

_:C_ELECTROSTATICS_SOLVER rdf:type owl:AllDifferent;
  owl:distinctMembers (viso-am:DIRECT_COULOMB_SUM viso-am:EWALD viso-am:EWALD_SMEARED viso-am:SPME viso-am:P3M).

# barostat

viso-am:LANGEVIN_BAROSTAT a viso-am:barostat;
  rdfs:seeAlso """Ask F. Jakobsen. Constant-pressure and constant-surface tension simulations in dissipative particle 
dynamics. Journal of Chemical Physics, 122(12):124901, 2005."""^^xs:string.

viso-am:BERENDSEN_BAROSTAT a viso-am:barostat;
  rdfs:seeAlso """H. J. C. Berendsen, J. P. M. Postma, W. F. van Gunsteren, A. DiNola, and J. R. Haak. Molecular
dynamics with coupling to an external bath. Journal of Chemical Physics, 81(8):3684–3690, 1984."""^^xs:string.

viso-am:PARRINELLO_RAHMAN_BAROSTAT a viso-am:barostat;
  rdfs:seeAlso "M. Parrinello and A. Rahman, J. Appl. Phys. https://doi.org/10.1063/1.328693 52, 7182 (1981)."^^xs:string.

_:C_BAROSTAT rdf:type owl:AllDifferent;
  owl:distinctMembers (viso-am:LANGEVIN_BAROSTAT viso-am:BERENDSEN_BAROSTAT viso-am:PARRINELLO_RAHMAN_BAROSTAT).

# parallelization_scheme

viso-am:DOMAIN_DECOMPOSITION a viso-am:parallelization_scheme.
viso-am:REPLICATED_DATA a viso-am:parallelization_scheme.

_:C_PARALLELIZATION_SCHEME rdf:type owl:AllDifferent;
  owl:distinctMembers (viso-am:REPLICATED_DATA viso-am:DOMAIN_DECOMPOSITION).

#sampling_algorithm

viso-am:METROPOLIS a viso-am:sampling_algorithm;
  rdfs:seeAlso"""N.A. Metropolis, A.W. Rosenbluth, M.N. Rosenbluth, A.H. Teller, E. Teller. 
  Equation of state calculations by fast computing machines. J. Chem. Phys., 21, 1087 (1953)."""^^xs:string.
viso-am:UMBRELLA_SAMPLING a viso-am:sampling_algorithm;
  rdfs:seeAlso"""G. M. Torrie and J. P. Valleau. Nonphysical sampling distributions in Monte Carlo free-energy estimation: Umbrella sampling. 
  J. Comput. Phys. 23, 187 (1977)."""^^xs:string.
viso-am:WANG_LANDAU_SAMPLING a viso-am:sampling_algorithm;
  rdfs:seeAlso"""Fugao Wang and D. P. Landau. Efficient, Multiple-Range Random Walk Algorithm to Calculate the Density of States. 
  Phys. Rev. Lett. 86, 2050 (2001)."""^^xs:string.

_:C_SAMPLING_ALGORITHM rdf:type owl:AllDifferent;
  owl:distinctMembers (viso-am:METROPOLIS viso-am:UMBRELLA_SAMPLING viso-am:WANG_LANDAU_SAMPLING).

#charge_smearing

viso-am:GAUSSIAN_SMEARING a viso-am:charge_smearing.
viso-am:SLATER_SMEARING a viso-am:charge_smearing.
viso-am:LINEAR_SMEARING a viso-am:charge_smearing.

_:C_CHARGE_SMEARING rdf:type owl:AllDifferent;
  owl:distinctMembers (viso-am:GAUSSIAN_SMEARING viso-am:SLATER_SMEARING viso-am:LINEAR_SMEARING).

# potential

# Van der Waals (potential)
# lennard_jones (potential)
viso-am:LENNARD_JONES_12_6 a viso-am:mie_potential. 
viso-am:BUCKINGHAM a viso-am:buckingham. 

# dpd_potential

viso-am:GROOT_WARREN a viso-am:dpd_potential;
  a viso-am:two_body_potential;
  rdfs:seeAlso "Robert D. Groot and Patrick B. Warren. Dissipative particle dynamics: Bridging the gap between atomistic and mesoscopic simulation. Journal of Chemical Physics, 107(11):4423–4435, 1997."^^xs:string.

viso-am:MANYBODY_DPD a viso-am:dpd_potential;
  rdfs:comment "Density-dependent pair-wise potential for Dissipative Particle Dynamics."^^xs:string;
  rdfs:seeAlso "I. Pagonabarraga and D. Frenkel. Dissipative particle dynamics for interacting systems. Journal of Chemical Physics, 115(11):5015–5026, 2001."^^xs:string.

_:C_DPD_POTENTIAL rdf:type owl:AllDifferent;
   owl:distinctMembers (viso-am:GROOT_WARREN viso-am:MANYBODY_DPD).

# non_conservative_force

viso-am:RANDOM_AND_DRAG_DPD_FORCE a viso-am:non_conservative_force;
  viso:is_modelling_twin_of viso-am:DPD_THERMOSTAT.

# electrostatic_potential

viso-am:COULOMB_POTENTIAL a viso-am:electrostatic_potential;
  rdfs:comment "Electrostatic potential between point charges."^^xs:string.

viso-am:CHARGE_DIPOLE_POTENTIAL a viso-am:electrostatic_potential;
  rdfs:comment "Electrostatic potential between a point charge and a point dipole."^^xs:string.

viso-am:DIPOLE_DIPOLE_POTENTIAL a viso-am:electrostatic_potential;
  rdfs:comment "Electrostatic potential between point charge dipoles."^^xs:string.

viso-am:CHARGE_QUADRUPOLE_POTENTIAL a viso-am:electrostatic_potential;
  rdfs:comment "Electrostatic potential between a point charge and a point charge quadrupole."^^xs:string.

viso-am:DIPOLE_QUADRUPOLE_POTENTIAL a viso-am:electrostatic_potential;
  rdfs:comment "Electrostatic potential between a point charge dipole and a point charge quadrupole."^^xs:string.

viso-am:QUADRUPOLE_QUADRUPOLE_POTENTIAL a viso-am:electrostatic_potential;
  rdfs:comment "Electrostatic potential between point charge quadrupoles."^^xs:string.

_:C_ELECTROSTATIC_POTENTIAL rdf:type owl:AllDifferent;
  owl:distinctMembers (viso-am:COULOMB_POTENTIAL viso-am:CHARGE_DIPOLE_POTENTIAL viso-am:DIPOLE_DIPOLE_POTENTIAL viso-am:CHARGE_QUADRUPOLE_POTENTIAL viso-am:DIPOLE_QUADRUPOLE_POTENTIAL viso-am:QUADRUPOLE_QUADRUPOLE_POTENTIAL).

# metal_potential

viso-am:FINNIS_SINCLAIR_POTENTIAL a viso-am:metal_potential;
    rdfs:seeAlso"Finnis, M. W., and Sinclair, J. E., A simple empirical N-body potential for transition metals. Philos. Mag. A, 50, 45 (1984)."^^xs:string.

# geometric_constraint

viso-am:RIGID_BOND a viso-am:geometric_constraint.

viso-am:RIGID_ANGLE a viso-am:geometric_constraint.

# geometric_constraint_algorithm

viso-am:SHAKE a viso-am:geometric_constraint_algorithm.

viso-am:RATTLE a viso-am:geometric_constraint_algorithm.

#boundary_condition

viso-am:NO_BOUNDARY a viso-am:boundary_condition.

viso-am:CUBIC_PERIODIC_BOUNDARY a viso-am:boundary_condition.

viso-am:ORTHOROMBIC_PERIODIC_BOUNDARY a viso-am:boundary_condition.

viso-am:LEES_EDWARDS_BOUNDARY_CONDITION a viso-am:boundary_condition;
  rdfs:comment "Lees-Edwards boundary condition allows to simulate a shear flow."^^xs:string;
  rdfs:seeAlso "A. W. Lees and S. F. Edwards. The computer study of transport processes under extreme conditions. J. Phys, C 5, 1921 (1972)."^^xs:string.

# combination_rule

viso-am:LORENTZ_BERTHELOT_COMBINATION_RULE a viso-am:combination_rule;
  rdfs:seeAlso "Lorentz, H. A. (1881), Ueber die Anwendung des Satzes vom Virial in der kinetischen Theorie der Gase. Ann. Phys., 248: 127-136."^^xs:string;
  rdfs:seeAlso "D. Berthelot, “Sur le mélange des gaz,” Comptes Rendus Hebdomadaires des Séances de l'Académie des Sciences, vol. 126, pp. 1703–1855, 1898."^^xs:string.
   
viso-am:GEOMETRIC_COMBINATION_RULE a viso-am:combination_rule.

_:C_COMBINATION_RULE rdf:type owl:AllDifferent;
  owl:distinctMembers (viso-am:LORENTZ_BERTHELOT_COMBINATION_RULE viso-am:GEOMETRIC_COMBINATION_RULE).

# planar_wall

viso-am:REFLECTING_PLANAR_HARD_WALL a viso-am:planar_wall;
  rdfs:comment "When a particle tries to cross such wall, its velocity component perperdicular to the wall is reversed."^^xs:string;
  rdfs:seeAlso "M. Revenga, I. Zúñiga, P. Español and I. Pagonabarraga. Boundary Models in DPD. Int. J. Mod. Phys. C 9, 1319 (1998)."^^xs:string;
  rdfs:seeAlso "P. B. Warren, P. Prinsen and M. A. J. Michels. The physics of surfactant dissolution. Phil. Trans. R. Soc Lond. A 361, 665 (2003)."^^xs:string.

viso-am:BOUNCE_BACK_PLANAR_HARD_WALL a viso-am:planar_wall;
  a viso:R_IS_MESOSCOPIC;
  rdfs:comment "When a particle tries to cross such wall, all its velocity components are reversed."^^xs:string;
  rdfs:seeAlso "M. Revenga, I. Zúñiga, P. Español and I. Pagonabarraga. Boundary Models in DPD. Int. J. Mod. Phys. C 9, 1319 (1998)."^^xs:string.

_:C_PLANAR_WALL rdf:type owl:AllDifferent;
  owl:distinctMembers (viso-am:REFLECTING_PLANAR_HARD_WALL viso-am:BOUNCE_BACK_PLANAR_HARD_WALL).

# site_surface_potential

viso-am:SOFT_REPULSIVE_WALL_POTENTIAL a viso-am:site_surface_potential;
  a viso:am_external_condition_trait;
  rdfs:seeAlso "P. B. Warren, P. Prinsen and M. A. J. Michels. The physics of surfactant dissolution. Phil. Trans. R. Soc Lond. A 361, 665 (2003)."^^xs:string;
  rdfs:comment "This soft repulsive potential can be used to decrease density oscillations near the wall."^^xs:string.
