@prefix : <http://matolab.org/ontology/container#> .
@prefix owl: <http://www.w3.org/2002/07/owl#> .
@prefix rdf: <http://www.w3.org/1999/02/22-rdf-syntax-ns#> .
@prefix xml: <http://www.w3.org/XML/1998/namespace> .
@prefix xsd: <http://www.w3.org/2001/XMLSchema#> .
@prefix moco: <http://matolab.org/ontology/container#> .
@prefix rdfs: <http://www.w3.org/2000/01/rdf-schema#> .
@base <http://matolab.org/ontology/container#> .

<http://matolab.org/ontology/container#> rdf:type owl:Ontology ;
                                          owl:versionIRI <https://gitlab.cc-asp.fraunhofer.de/fraunhofer-iwm-hub-materialdigital/semantic-containers/-/raw/master/ontologies/moco.owl> ;
                                          owl:imports <http://purl.org/co> ;
                                          <http://purl.org/dc/elements/1.1/contributor> "Fraunhofer IWM, DE" ;
                                          <http://purl.org/dc/elements/1.1/creator> "Akhil Thomas" ,
                                                                                    "Elena Trelles" ,
                                                                                    "Philipp von Hartrott" ,
                                                                                    "Sascha Fliegner" ;
                                          rdfs:comment "This ontology is released under a Creative Commons license Attribution 4.0 International (CC BY 4.0)" ;
                                          owl:versionInfo "1.0.0" .

#################################################################
#    Object Properties
#################################################################

###  http://matolab.org/ontology/container#mol_00001
moco:mol_00001 rdf:type owl:ObjectProperty ;
               rdfs:subPropertyOf owl:topObjectProperty ;
               rdfs:range <http://purl.org/co/List> ;
               rdfs:comment """This property points to a http://pur.org/co/list whose items are lists again. The first level of lists represent the tables inside the container while the second level of lists represent the individual columns of a table. 

The tables (aka dataset) in the HDF5 container are accessed throught their (1-based) index (converted to a string). The columns of a table are accessed through their (1-based) numeric column index.

The type of the values in a specific column is represented by a \"sample value\" given as a list item content (property: has_item_content). This assumes that the type is composed of a value (given in the column/cell) and other properties e.g. like dimension and physical unit. The quantityValue type from Wikibase is an example for this.""" ;
               rdfs:label "has dataset description"@de .


#################################################################
#    Data properties
#################################################################

###  http://matolab.org/ontology/container#mol_00002
moco:mol_00002 rdf:type owl:DatatypeProperty ;
               rdfs:subPropertyOf owl:topDataProperty ;
               rdfs:range xsd:anyURI ;
               rdfs:comment "The value of this literal is a URL from which a file should be downloadable using the protocol specified in the URL."@en ;
               rdfs:label "URL_to_file"@de .


#################################################################
#    Classes
#################################################################

###  http://matolab.org/ontology/container#mol_00003
moco:mol_00003 rdf:type owl:Class ;
               rdfs:subClassOf [ rdf:type owl:Restriction ;
                                 owl:onProperty moco:mol_00002 ;
                                 owl:someValuesFrom xsd:anyURI
                               ] ;
               rdfs:comment "Instances of  this class repesent a HDF5 based container in a knowledge graph. The URL_to_file should point to a URL from which the actual HDF5 file can be downloaded, given the access restrictions are fulfilled."@en ;
               rdfs:label "HDF5_Container_for_series"@de .


###  Generated by the OWL API (version 4.5.9.2019-02-01T07:24:44Z) https://github.com/owlcs/owlapi
